

STAT 5244 – Unsupervised Learning

Homework 2

Name: Chuyang Su UNI: cs4570

1 Mixture Models

1.1 EM Algorithm Derivation

Since we model count-valued data, assume each observation $x_i = (x_{i1}, \dots, x_{ip}) \in \mathbb{N}_0^p$ is generated from a finite mixture of *independent* Poisson distributions:

$$p(x_i; \pi, \lambda) = \sum_{k=1}^K \pi_k \prod_{j=1}^p \frac{e^{-\lambda_{kj}} \lambda_{kj}^{x_{ij}}}{x_{ij}!}, \quad \pi_k \geq 0, \quad \sum_{k=1}^K \pi_k = 1, \quad \lambda_{kj} > 0.$$

Here $\pi = (\pi_1, \dots, \pi_K)$ are mixture weights and $\lambda_k = (\lambda_{k1}, \dots, \lambda_{kp})$ are component-wise Poisson means.

Latent variables. Introduce latent indicators $z_{ik} \in \{0, 1\}$ with $\sum_{k=1}^K z_{ik} = 1$, where $z_{ik} = 1$ if x_i comes from component k . The complete-data likelihood is

$$L_c(\pi, \lambda) = \prod_{i=1}^n \prod_{k=1}^K \left[\pi_k \prod_{j=1}^p \frac{e^{-\lambda_{kj}} \lambda_{kj}^{x_{ij}}}{x_{ij}!} \right]^{z_{ik}}.$$

Taking logs and dropping constants independent of (π, λ) (i.e., $\log x_{ij}!$) gives the complete-data log-likelihood

$$\ell_c(\pi, \lambda) \propto \sum_{i=1}^n \sum_{k=1}^K z_{ik} \left[\log \pi_k + \sum_{j=1}^p (x_{ij} \log \lambda_{kj} - \lambda_{kj}) \right].$$

E-step Derivation. Since the latent indicators z_{ik} are unobserved, we take their conditional expectation under the current parameters. Define

$$\gamma_{ik} := \mathbb{E}[z_{ik} \mid x_i; \pi^{(t)}, \lambda^{(t)}] = P(z_{ik} = 1 \mid x_i; \pi^{(t)}, \lambda^{(t)}),$$

which represents the posterior probability that observation x_i belongs to component k .

Using Bayes' theorem,

$$P(z_{ik} = 1 \mid x_i; \pi^{(t)}, \lambda^{(t)}) = \frac{P(z_{ik} = 1; \pi^{(t)}) P(x_i \mid z_{ik} = 1; \lambda^{(t)})}{P(x_i; \pi^{(t)}, \lambda^{(t)})}.$$

Each term can be expressed as:

$$P(z_{ik} = 1; \pi^{(t)}) = \pi_k^{(t)}, \quad P(x_i \mid z_{ik} = 1; \lambda^{(t)}) = \prod_{j=1}^p \frac{e^{-\lambda_{kj}^{(t)}} (\lambda_{kj}^{(t)})^{x_{ij}}}{x_{ij}!},$$

and

$$P(x_i; \pi^{(t)}, \lambda^{(t)}) = \sum_{\ell=1}^K \pi_{\ell}^{(t)} \prod_{j=1}^p \frac{e^{-\lambda_{\ell j}^{(t)}} (\lambda_{\ell j}^{(t)})^{x_{ij}}}{x_{ij}!}.$$

Substituting these expressions into Bayes' rule yields:

$$\gamma_{ik} = \frac{\pi_k^{(t)} \prod_{j=1}^p e^{-\lambda_{kj}^{(t)}} (\lambda_{kj}^{(t)})^{x_{ij}} / x_{ij}!}{\sum_{\ell=1}^K \pi_{\ell}^{(t)} \prod_{j=1}^p e^{-\lambda_{\ell j}^{(t)}} (\lambda_{\ell j}^{(t)})^{x_{ij}} / x_{ij}!}.$$

Since the term $\prod_{j=1}^p x_{ij}!$ does not depend on k , it cancels out between numerator and denominator. Therefore, the final expression for the responsibilities is:

$$\gamma_{ik} = \frac{\pi_k^{(t)} \prod_{j=1}^p e^{-\lambda_{kj}^{(t)}} (\lambda_{kj}^{(t)})^{x_{ij}}}{\sum_{\ell=1}^K \pi_{\ell}^{(t)} \prod_{j=1}^p e^{-\lambda_{\ell j}^{(t)}} (\lambda_{\ell j}^{(t)})^{x_{ij}}}, \quad i = 1, \dots, n, \quad k = 1, \dots, K.$$

M-step. We maximize

$$Q(\pi, \lambda) = \sum_{i=1}^n \sum_{k=1}^K \gamma_{ik} \left[\log \pi_k + \sum_{j=1}^p (x_{ij} \log \lambda_{kj} - \lambda_{kj}) \right]$$

subject to $\pi_k \geq 0$, $\sum_{k=1}^K \pi_k = 1$, and $\lambda_{kj} > 0$.

Update for π_k . Introduce a Lagrange multiplier η for the simplex constraint:

$$\mathcal{L}(\pi, \eta) = \sum_{k=1}^K \left(\sum_{i=1}^n \gamma_{ik} \right) \log \pi_k + \eta \left(1 - \sum_{k=1}^K \pi_k \right).$$

Setting the partial derivatives to zero,

$$\frac{\partial \mathcal{L}}{\partial \pi_k} = \frac{\sum_{i=1}^n \gamma_{ik}}{\pi_k} - \eta = 0 \quad \implies \quad \pi_k = \frac{\sum_{i=1}^n \gamma_{ik}}{\eta}.$$

Summing over k and using $\sum_{k=1}^K \pi_k = 1$ gives

$$1 = \sum_{k=1}^K \pi_k = \frac{1}{\eta} \sum_{k=1}^K \sum_{i=1}^n \gamma_{ik} = \frac{1}{\eta} \sum_{i=1}^n \sum_{k=1}^K \gamma_{ik} = \frac{1}{\eta} \sum_{i=1}^n 1 = \frac{n}{\eta} \implies \eta = n.$$

Hence

$$\pi_k^{(t+1)} = \frac{1}{n} \sum_{i=1}^n \gamma_{ik}.$$

(Concavity: $\partial^2 \mathcal{L} / \partial \pi_k^2 = -(\sum_i \gamma_{ik}) / \pi_k^2 < 0$.)

Update for λ_{kj} . For each (k, j) , the terms of Q that involve λ_{kj} are

$$Q_{kj}(\lambda_{kj}) = \sum_{i=1}^n \gamma_{ik} (x_{ij} \log \lambda_{kj} - \lambda_{kj}).$$

Differentiate and set to zero:

$$\frac{\partial Q_{kj}}{\partial \lambda_{kj}} = \sum_{i=1}^n \gamma_{ik} \left(\frac{x_{ij}}{\lambda_{kj}} - 1 \right) = 0 \quad \implies \quad \lambda_{kj} = \frac{\sum_{i=1}^n \gamma_{ik} x_{ij}}{\sum_{i=1}^n \gamma_{ik}}.$$

(Concavity: $\partial^2 Q_{kj} / \partial \lambda_{kj}^2 = -\sum_i \gamma_{ik} x_{ij} / \lambda_{kj}^2 < 0$ when $\lambda_{kj} > 0$.) Therefore

$$\lambda_{kj}^{(t+1)} = \frac{\sum_{i=1}^n \gamma_{ik} x_{ij}}{\sum_{i=1}^n \gamma_{ik}}.$$

A Appendix: Code Implementation